$ d(\frac{(sin((2 \cdot x+3)))^3}{cos(x)}) = \frac{d((sin((2 \cdot x+3)))^3) \cdot (cos(x)) + d(cos(x)) \cdot ((sin((2 \cdot x+3)))^3)}{cos(x)}$

Посчитаем составные части:

$ d(cos(x)) = (-1) \cdot sin(x) \cdot d(x)$

Посчитаем составные части:

$ d(x) = 1$

Получилось:

$ d(cos(x)) = -1 \cdot sin(x)$

$ d((sin((2 \cdot x+3)))^3) = 3 \cdot (sin((2 \cdot x+3)))^(3 - 1) \cdot d(sin((2 \cdot x+3)))$

Посчитаем составные части:

$ d(sin((2 \cdot x+3))) = cos((2 \cdot x+3)) \cdot d((2 \cdot x+3))$

Посчитаем составные части:

$ d((2 \cdot x+3)) = d(2 \cdot x) + d(3)$

Посчитаем составные части:

$ d(3) = 0$

$ d(2 \cdot x) = d(2) \cdot (x) + d(x) \cdot (2)$

Посчитаем составные части:

$ d(x) = 1$

$ d(2) = 0$

Получилось:

$ d(2 \cdot x) = 2$

Получилось:

$ d((2 \cdot x+3)) = 2$

Получилось:

$ d(sin((2 \cdot x+3))) = cos((2 \cdot x+3)) \cdot 2$

Получилось:

$ d((sin((2 \cdot x+3)))^3) = 3 \cdot (sin((2 \cdot x+3)))^2 \cdot cos((2 \cdot x+3)) \cdot 2$

Получилось:

$ d(\frac{(sin((2 \cdot x+3)))^3}{cos(x)}) = \frac{(3 \cdot (sin((2 \cdot x+3)))^2 \cdot cos((2 \cdot x+3)) \cdot 2 \cdot cos(x)-(sin((2 \cdot x+3)))^3 \cdot -1 \cdot sin(x))}{cos(x) \cdot cos(x)}$

